src/impl/TLS13.Impl.ConnectionState.LocalHandshake.fst
@@ -615,6 +615,7 @@ fn select_server_parameters
     c.handshake.messages.client_hello_cipher_suites_len
     c.handshake.messages.client_hello_signature_schemes_len
     c.handshake.messages.client_hello_session_id_len
+    c.handshake.messages.client_hello_kex_group
     st0.CS.cs_model.CS.model_handshake.CS.hs_client_hello) as
     (client_hello_metadata_exactly
       c.handshake.messages.client_hello_has_server_name
@@ -622,6 +623,7 @@ fn select_server_parameters
       c.handshake.messages.client_hello_cipher_suites_len
       c.handshake.messages.client_hello_signature_schemes_len
       c.handshake.messages.client_hello_session_id_len
+      c.handshake.messages.client_hello_kex_group
       (selected_server_parameters_state st0 (Ghost.reveal selection)).CS.cs_model.CS.model_handshake.CS.hs_client_hello);
   fold (handshake_messages_exactly
     c.handshake.messages
@@ -772,6 +774,7 @@ fn select_server_parameters_with_private_from_array
     c.handshake.messages.client_hello_cipher_suites_len
     c.handshake.messages.client_hello_signature_schemes_len
     c.handshake.messages.client_hello_session_id_len
+    c.handshake.messages.client_hello_kex_group
     st0.CS.cs_model.CS.model_handshake.CS.hs_client_hello) as
     (client_hello_metadata_exactly
       c.handshake.messages.client_hello_has_server_name
@@ -779,6 +782,7 @@ fn select_server_parameters_with_private_from_array
       c.handshake.messages.client_hello_cipher_suites_len
       c.handshake.messages.client_hello_signature_schemes_len
       c.handshake.messages.client_hello_session_id_len
+      c.handshake.messages.client_hello_kex_group
       (selected_server_parameters_state st0 (Ghost.reveal selection)).CS.cs_model.CS.model_handshake.CS.hs_client_hello);
   fold (handshake_messages_exactly
     c.handshake.messages
@@ -2656,6 +2660,7 @@ fn try_send_client_hello
       c.handshake.messages.client_hello_cipher_suites_len
       c.handshake.messages.client_hello_signature_schemes_len
       c.handshake.messages.client_hello_session_id_len
+      c.handshake.messages.client_hello_kex_group
       st0.CS.cs_model.CS.model_handshake.CS.hs_client_hello);
     with old_ch_has_server_name old_ch_server_name_len
          old_ch_cipher_suites_len old_ch_signature_schemes_len. _;
@@ -2888,6 +2893,7 @@ fn try_send_client_hello
       c.handshake.messages.client_hello_cipher_suites_len
       c.handshake.messages.client_hello_signature_schemes_len
       c.handshake.messages.client_hello_session_id_len
+      c.handshake.messages.client_hello_kex_group
       (Some (Ghost.reveal ch)));
     fold (handshake_messages_exactly
       c.handshake.messages
